Projection of traces to a subset of nodes (with no-equivocation constraint)

VLSM/SubProjectionTraces.v
@@ -2,15 +2,14 @@ Require Import List Nat Bool.
 Import ListNotations.
 Require Import Lia.
 Require Import Logic.FunctionalExtensionality.
+Require Import Program.
 
 Require Import Coq.Logic.FinFun Coq.Logic.Eqdep.
 
 From CasperCBC
-Require Import Lib.ListExtras Lib.Preamble VLSM.Common VLSM.Composition.
+Require Import Lib.ListExtras Lib.Preamble VLSM.Common VLSM.Composition VLSM.Equivocation.
 
-Section SubProjectionTraces.
-
-Print sub_IM.
+Section sub_composition.
 
 Context
   {message : Type}
@@ -19,20 +18,87 @@ Context
   (IM : index -> VLSM message)
   (sub_index_list : list index)
   (Hi0_sub : sub_index_list <> [])
-  (sub_index : Type := sub_index sub_index_list)
-  (sub_index_eq_dec := sub_index_eq_dec sub_index_list)
-  (sub_index_prop := sub_index_prop sub_index_list)
-  (sub_index_prop_dec := sub_index_prop_dec sub_index_list)
-  (sub_IM : sub_index -> VLSM message := sub_IM IM sub_index_list)
   .
 
-Existing Instance sub_index_prop_dec.
+Definition sub_index_prop (i : index) : Prop := In i sub_index_list.
+
+Local Instance sub_index_prop_dec
+  (i : index)
+  : Decision (sub_index_prop i).
+Proof.
+  apply in_dec. assumption.
+Qed.
+
+Definition sub_index : Type
+  := dec_sig sub_index_prop.
+
+Local Instance sub_index_i0 : Inhabited sub_index.
+Proof.
+  split.
+  destruct (destruct_list sub_index_list) as [[x [tl Heq]]| n]
+  ; [|elim Hi0_sub; assumption].
+  exists x. apply bool_decide_eq_true.
+  unfold sub_index_prop. subst sub_index_list. left. reflexivity.
+Qed.
+
+Local Instance sub_index_eq_dec : EqDecision sub_index.
+Proof.
+  apply dec_sig_eq_dec. assumption.
+Qed.
+
+Definition sub_IM
+  (ei : sub_index)
+  : VLSM message
+  := IM (proj1_sig ei).
+
+ Lemma sub_IM_state_update_eq
+  (i : index)
+  (s : composite_state sub_IM)
+  (si : vstate (IM i))
+  (e1 e2 : sub_index_prop i)
+  : state_update sub_IM s (dec_exist _ i e1) si (dec_exist _ i e2) = si.
+Proof.
+  unfold dec_exist.
+  assert
+    (forall be1 be2, be1 = be2 -> state_update sub_IM s
+      (exist _ i be1) si (exist _ i be2)
+      = si).
+  { intros. subst. apply state_update_eq. }
+  apply H.
+  apply bool_decide_eq_true_proof_irrelevance.
+Qed.
+ 
+
+Definition free_sub_vlsm_composition : VLSM message
+  := free_composite_vlsm sub_IM.
+
+Definition seeded_free_sub_composition
+  (messageSet : message -> Prop)
+  := pre_loaded_with_vlsm free_sub_vlsm_composition
+      (fun m => messageSet m \/ composite_initial_message_prop IM m).
+
+Local Lemma i0 : Inhabited index.
+Proof.
+  apply exists_last in Hi0_sub.
+  destruct Hi0_sub as (_, (a, _)).
+  constructor. exact a.
+Qed.
+
+Existing Instance i0.
 
 Definition composite_state_sub_projection
   (s : composite_state IM)
   (subi : sub_index)
   : vstate (sub_IM subi)
   := s (proj1_sig subi).
+
+Lemma composite_initial_state_sub_projection
+  (s : composite_state IM)
+  (Hs : composite_initial_state_prop IM s)
+  : composite_initial_state_prop sub_IM (composite_state_sub_projection s).
+Proof.
+  intros (i, Hi). apply Hs.
+Qed.
 
 Definition composite_transition_item_sub_projection
   (item : composite_transition_item IM)
@@ -43,6 +109,17 @@ Definition composite_transition_item_sub_projection
   :=
   @Build_transition_item _ (composite_type sub_IM) (existT _ j (projT2 (l item))) (input item) (composite_state_sub_projection (destination item)) (output item).
 
+Lemma composite_state_transition_item_sub_projection
+  (item : composite_transition_item IM)
+  (i := projT1 (l item))
+  (e : sub_index_prop i)
+  (j : sub_index := dec_exist _ i e)
+  : composite_state_sub_projection (destination item)
+  = destination (composite_transition_item_sub_projection item e).
+Proof.
+  destruct item. destruct l. simpl in *. reflexivity.
+Qed.
+
 Definition composite_transition_item_sub_projection_proof_irrelevance
   (item : composite_transition_item IM)
   (i := projT1 (l item))
@@ -52,17 +129,9 @@ Proof.
   destruct item. destruct l. unfold i in *. clear i.
   unfold composite_transition_item_sub_projection.
   simpl in *. f_equal.
-  match goal with
-  |- existT _ ?x1 _ = existT _ ?x2 _ => assert (Heq : x1 = x2)
-  end.
-  { apply dec_sig_eq_iff. reflexivity. }
-  simpl in *.
-  rewrite Heq.
-  assert (Heq : dec_exist sub_index_prop x e1 = dec_exist sub_index_prop x e2)
-  ; [|rewrite Heq].
-  unfold dec_exist. rewrite decide_True.
-  assert (dec_exist sub_index_prop x e1)
-
+  apply (@dec_sig_sigT_eq _ sub_index_prop sub_index_prop_dec (fun i => vlabel (IM i))).
+  reflexivity.
+Qed.
 
 Definition from_sub_projection
   (a : composite_transition_item IM)
@@ -95,126 +164,109 @@ Definition finite_trace_sub_projection_alt
     )
   (list_annotate from_sub_projection ftrx Hall).
 
-Lemma finite_trace_sub_projection_alt_cons
-  (item : composite_transition_item IM)
-  (trx : list (composite_transition_item IM))
-  : finite_trace_sub_projection_alt (item :: trx) =
-    let tail := finite_trace_sub_projection_alt trx in
-    match decide (from_sub_projection item) with
-    | left e => composite_transition_item_sub_projection item e :: tail
-    | _ => tail
-    end.
-Proof.
-  unfold finite_trace_sub_projection_alt at 1.
-  match goal with 
-  |- context [list_annotate _ _ ?all] =>
-    remember all as Hall
-  end.
-  clear HeqHall.
-  match goal with 
-  |- context [list_annotate _ ?f _] =>
-    remember f as flt
-  end.
-  simpl in Heqflt.
-  unfold bool_decide in Heqflt at 1.
-  unfold decide.
-  destruct (sub_index_prop_dec (projT1 (l item))) eqn:Hitem.
-  - subst flt.
-    rewrite list_annotate_unroll.
-    rewrite map_cons.
-  ; [|subst; reflexivity].
-  destruct (dec)
-  change (item :: trx) with ([item] ++ trx).
-  rewrite (filter_app _ [item] trx).
-  unfold filter.
-
-Lemma finite_trace_projection_list_alt_iff
+Lemma finite_trace_sub_projection_alt_iff
   (trx : list (composite_transition_item IM))
   : finite_trace_sub_projection_alt trx = finite_trace_sub_projection trx.
 Proof.
+  unfold finite_trace_sub_projection_alt.
+  match goal with
+  |- context [list_annotate _ _ ?H] => generalize H as Hall
+  end.
   induction trx; intros; [reflexivity|].
-  simpl.
-  destruct
-    (decide (from_sub_projection a)) eqn:Heq.
-      j =
-    (@projT1 index (fun n : index => @vlabel message (IM n))
-       (@l message (@composite_type message index IM) a))))
-    eqn:Heq.
-  - assert
-    (Hunroll :
-      filter (fun a => bool_decide (from_projection a)) (a :: trx)
-      = a :: filter (fun a => bool_decide (from_projection a)) trx
-    ).
-    { simpl.
-      unfold bool_decide, dec_from_projection, from_projection.
-      replace
-        (decide (j =
-        (@projT1 index (fun n : index => @vlabel message (IM n))
-           (@l message (@type message X) a))))
-      with
-        (@left
-           (@eq index j
-              (@projT1 index (fun n : index => @vlabel message (IM n))
-                 (@l message (@composite_type message index IM) a)))
-           (not
-              (@eq index j
-                 (@projT1 index (fun n : index => @vlabel message (IM n))
-                    (@l message (@composite_type message index IM) a)))) e)
-      .
-      reflexivity.
-    }
-    unfold finite_trace_projection_list_alt.
-    generalize dependent Hall.
-    rewrite Hunroll.
-    intro Hall.
-    rewrite list_annotate_unroll.
-    specialize (IHtrx (Forall_tl Hall)).
-    rewrite <- IHtrx.
-    simpl.
+  simpl. unfold bool_decide at 1. unfold decide.
+  simpl in Hall. unfold bool_decide in Hall at 1.
+  destruct (sub_index_prop_dec (projT1 (l a))) eqn:Ha.
+  - rewrite list_annotate_unroll.
+    rewrite map_cons.
     f_equal.
-    f_equal; try reflexivity.
-    replace (Forall_hd Hall) with e; try reflexivity.
-    apply UIP.
-  - assert
-    (Hunroll :
-      filter (fun a => bool_decide (from_projection a)) (a :: trx)
-      = filter (fun a => bool_decide (from_projection a)) trx
-    ).
-    { simpl.
-      unfold bool_decide, dec_from_projection, from_projection.
-      replace
-        (decide (j =
-        (@projT1 index (fun n0 : index => @vlabel message (IM n0))
-           (@l message (@type message X) a))))
-      with
-        (@right
-          (@eq index j
-             (@projT1 index (fun n : index => @vlabel message (IM n))
-                (@l message (@composite_type message index IM) a)))
-          (not
-             (@eq index j
-                (@projT1 index (fun n : index => @vlabel message (IM n))
-                   (@l message (@composite_type message index IM) a)))) n)
-        .
-      reflexivity.
-    }
-    unfold finite_trace_projection_list_alt.
-    generalize dependent Hall.
-    rewrite Hunroll.
-    intro Hall.
-    specialize (IHtrx Hall).
-    rewrite <- IHtrx.
-    reflexivity.
+    +  apply composite_transition_item_sub_projection_proof_irrelevance.
+    + apply IHtrx.
+  - apply IHtrx.
 Qed.
 
-Lemma finite_trace_projection_empty
-  (s : vstate X)
-  (trx : list (vtransition_item X))
+Section sub_projection_with_no_equivocation_constraints.
+
+Existing Instance  IndEqDec.
+
+Context
+  (constraint : composite_label IM -> composite_state IM * option message -> Prop)
+  (has_been_sent_capabilities : forall i : index, (has_been_sent_capability (IM i)))
+  {index_listing : list index}
+  (finite_index : Listing index_listing)
+  (Free := free_composite_vlsm IM)
+  (Sub_Free := free_composite_vlsm sub_IM)
+  (X_has_been_sent_capability : has_been_sent_capability Free := composite_has_been_sent_capability IM (free_constraint IM) finite_index has_been_sent_capabilities)
+  (X := composite_vlsm IM constraint)
+  (Pre := pre_loaded_with_all_messages_vlsm (free_composite_vlsm IM))
+  .
+
+Lemma sub_has_been_sent_capabilities : forall i : sub_index, (has_been_sent_capability (sub_IM i)).
+Proof.
+  intros [i Hi]. apply has_been_sent_capabilities.
+Qed.
+
+Fixpoint select_sub_indices
+  (l : list index)
+  : list sub_index
+  :=
+  match l with
+  | [] => []
+  | h :: t =>
+    let t' := select_sub_indices t in
+    match decide (sub_index_prop h) with
+    | left e => dec_exist _ h e :: t'
+    | _ => t'
+    end
+  end.
+
+Definition sub_index_listing : list sub_index := select_sub_indices index_listing.
+
+Lemma in_select_sub_indices
+  (a: index)
+  (s: sub_index_prop a)
+  (l: list index)
+  : In (dec_exist sub_index_prop a s) (select_sub_indices l) <-> In a l.
+Proof.
+  induction l; [simpl; intuition|].
+  simpl.
+  destruct (decide (sub_index_prop a0)); [|rewrite IHl].
+  - split; intros [Heq | H]; [left |right; apply IHl; assumption| left |right; apply IHl; assumption].
+    + apply dec_sig_eq_iff in Heq. assumption.
+    + apply dec_sig_eq_iff. assumption.
+  - split; [intuition|].
+    intros [Heq | H]; [|assumption].
+    subst. contradiction.
+Qed.
+
+Lemma finite_sub_index : Listing sub_index_listing.
+Proof.
+  unfold sub_index_listing.
+  clear -finite_index.
+  destruct finite_index as [Hnodup Hfinite].
+  split.
+  - clear Hfinite finite_index. induction index_listing; [constructor|].
+    inversion Hnodup. subst.
+    simpl. spec IHl H2.
+    destruct (decide (sub_index_prop a)); [|assumption].
+    constructor; [|assumption].
+    intro contra. elim H1. apply in_select_sub_indices in contra. assumption.
+  - intros subi. unfold sub_index in subi. destruct_dec_sig subi i Hi Heq.
+    subst. apply in_select_sub_indices. apply Hfinite.
+Qed.
+
+Local Instance Sub_Free_has_been_sent_capability
+  : has_been_sent_capability Sub_Free
+  :=
+  composite_has_been_sent_capability sub_IM (free_constraint sub_IM) finite_sub_index sub_has_been_sent_capabilities.
+
+Lemma finite_trace_sub_projection_empty
+  (s : composite_state IM)
+  (trx : list (composite_transition_item IM))
   (Htr : finite_protocol_trace_from X s trx)
-  (Hempty : finite_trace_projection_list trx = [])
+  (Hempty : finite_trace_sub_projection trx = [])
   (t : (vtransition_item X))
   (Hin : In t trx)
-  : destination t j = s j.
+  : forall j, In j sub_index_list -> destination t j = s j.
 Proof.
   generalize dependent t.
   induction Htr; simpl; intros t Hin.
@@ -224,18 +276,29 @@ Proof.
     unfold transition in Htransition; simpl in Htransition.
     destruct (vtransition (IM i) l (s' i, iom)) as [si' om'] eqn:Hteq.
     inversion Htransition; subst. clear Htransition.
-    destruct Hin as [Heq | Hin]; subst; simpl in *; destruct (decide (j = i)).
-    + inversion Hempty.
-    + apply state_update_neq. assumption.
-    + inversion Hempty.
-    + specialize (IHHtr Hempty t Hin). rewrite IHHtr.
-      apply state_update_neq. assumption.
+    match type of Hempty with
+      | finite_trace_sub_projection (?i :: _) = _ => remember i as item
+    end.
+    simpl in Hempty.
+    destruct (decide (from_sub_projection item))
+    ; [inversion Hempty|].
+    specialize (IHHtr Hempty).
+    rewrite Heqitem in n.
+    unfold from_sub_projection in n.
+    simpl in n.
+    destruct Hin as [Heq | Hin]; intros j Hj.
+    + subst. simpl. apply state_update_neq.
+      intro contra. subst. contradiction.
+    + assert (Hji : j <> i).
+      { intro contra. subst. contradiction. }
+      specialize (IHHtr _ Hin j Hj).
+      rewrite state_update_neq in IHHtr; assumption.
 Qed.
 
-Lemma finite_trace_projection_list_app
+Lemma finite_trace_sub_projection_app
   (tr1 tr2 : list (composite_transition_item IM))
-  : finite_trace_projection_list (tr1 ++ tr2) =
-    finite_trace_projection_list tr1 ++ finite_trace_projection_list tr2.
+  : finite_trace_sub_projection (tr1 ++ tr2) =
+    finite_trace_sub_projection tr1 ++ finite_trace_sub_projection tr2.
 Proof.
   induction tr1;[reflexivity|].
   simpl.
@@ -246,711 +309,385 @@ Proof.
   simpl. rewrite IHtr1. reflexivity.
 Qed.
 
-Lemma preloaded_finite_trace_projection_last_state
-  (start : vstate X)
-  (transitions : list (vtransition_item X))
-  (Htr : finite_protocol_trace_from (pre_loaded_with_all_messages_vlsm X) start transitions)
+Lemma finite_trace_sub_projection_list_in
+  (tr : list (composite_transition_item IM))
+  (itemX : composite_transition_item IM)
+  (HitemX : In itemX tr)
+  (j := projT1 (l itemX))
+  (Hj : sub_index_prop j)
+  : In (composite_transition_item_sub_projection itemX Hj) (finite_trace_sub_projection tr).
+Proof.
+  apply in_split in HitemX.
+  destruct HitemX as [pre [suf HitemX]].
+  subst.
+  change (itemX :: suf) with ([itemX] ++ suf).
+  rewrite! finite_trace_sub_projection_app.
+  apply in_app_iff. right. apply in_app_iff. left.
+  simpl. destruct (decide (from_sub_projection itemX)); [|contradiction].
+  left. apply composite_transition_item_sub_projection_proof_irrelevance.
+Qed.
+
+Lemma finite_trace_sub_projection_list_in_rev
+  (tr : list (composite_transition_item IM))
+  (j : index)
+  (itemj : composite_transition_item sub_IM)
+  (Hitemj : In itemj  (finite_trace_sub_projection tr))
+  : exists
+    (itemX : composite_transition_item IM)
+    (HitemX : from_sub_projection itemX),
+    In itemX tr /\ composite_transition_item_sub_projection itemX HitemX = itemj.
+Proof.
+  rewrite <- finite_trace_sub_projection_alt_iff in Hitemj.
+  apply in_map_iff in Hitemj.
+  destruct Hitemj as [(itemX, HitemX) [Heq Hin]].
+  exists itemX, HitemX.
+  split; [|assumption].
+  apply in_list_annotate_forget in Hin.
+  apply filter_In in Hin. apply Hin.
+Qed.
+
+Lemma preloaded_finite_trace_sub_projection_last_state
+  (start : composite_state IM)
+  (transitions : list (composite_transition_item IM))
+  (Htr : finite_protocol_trace_from Pre start transitions)
   (lstx := last (List.map destination transitions) start)
-  (lstj := last (List.map destination (finite_trace_projection_list transitions)) (start j))
-  : lstj = lstx j.
+  (lstj := last (List.map destination (finite_trace_sub_projection transitions)) (composite_state_sub_projection start))
+  : lstj = composite_state_sub_projection lstx.
 Proof.
   unfold lstx. unfold lstj. clear lstx. clear lstj.
-  induction Htr; try reflexivity.
-  destruct l as [i l].
+  induction Htr; [reflexivity|].
+  match goal with
+  |- context[finite_trace_sub_projection (?i :: _)] => remember i as item
+  end.
   rewrite map_cons.
   rewrite unroll_last. simpl.
-  destruct (decide (j = i)).
-  - rewrite map_cons. rewrite unroll_last.
+  destruct (decide (from_sub_projection item)).
+  - subst. rewrite map_cons. rewrite unroll_last.
     assumption.
   - destruct H as [[[_om Hs'] [[_s Hiom] Hvalid]] Htransition].
     unfold transition in Htransition; simpl in Htransition.
     unfold vtransition in Htransition. simpl in Htransition.
+    destruct l as (i, l).
     destruct (vtransition (IM i) l (s' i, iom)) as [si' om'] eqn:Hteq.
     inversion Htransition; subst. clear Htransition.
-    specialize (state_update_neq _ s' i si' j n); intro Hupd.
-    rewrite Hupd in *.
-    assumption.
+    simpl.
+    unfold from_sub_projection in n. simpl in n.
+    simpl in *.
+    rewrite <- IHHtr. f_equal.
+    apply functional_extensionality_dep_good.
+    intros (j, Hj). unfold composite_state_sub_projection.
+    simpl. symmetry. apply (state_update_neq _ s').
+    apply bool_decide_eq_true_1 in Hj.
+    intro contra. subst. contradiction. 
 Qed.
 
-Lemma finite_trace_projection_last_state
-  (start : vstate X)
-  (transitions : list (vtransition_item X))
+Lemma X_incl_Pre : VLSM_incl X Pre.
+Proof.
+  apply VLSM_incl_trans with (machine (free_composite_vlsm IM)).
+  - apply (constraint_free_incl IM constraint).
+  - apply vlsm_incl_pre_loaded_with_all_messages_vlsm.
+Qed.
+
+Lemma finite_trace_sub_projection_last_state
+  (start : composite_state IM)
+  (transitions : list (composite_transition_item IM))
   (Htr : finite_protocol_trace_from X start transitions)
   (lstx := last (List.map destination transitions) start)
-  (lstj := last (List.map destination (finite_trace_projection_list transitions)) (start j))
-  : lstj = lstx j.
+  (lstj := last (List.map destination (finite_trace_sub_projection transitions)) (composite_state_sub_projection start))
+  : lstj = composite_state_sub_projection lstx.
 Proof.
-  apply preloaded_finite_trace_projection_last_state.
-  apply VLSM_incl_finite_trace; [|assumption].
-  apply vlsm_incl_pre_loaded_with_all_messages_vlsm.
+  apply preloaded_finite_trace_sub_projection_last_state.
+  apply VLSM_incl_finite_trace with (machine X); [|assumption].
+  apply X_incl_Pre.
 Qed.
 
-Local Lemma _finite_ptrace_projection
-  (s : vstate X)
-  (Psj : protocol_state_prop Xj (s j))
-  (trx : list (vtransition_item X))
-  (Htr : finite_protocol_trace_from X s trx)
-   : finite_protocol_trace_from Xj (s j) (finite_trace_projection_list trx).
-Proof.
-  induction Htr.
-  - constructor. assumption.
-  - destruct l as [x lx]; simpl.
-    destruct H as [[Ps' [Piom [Hv Hc]]] Ht].
-    assert (Hpp : protocol_prop X (s, oom)).
-    { rewrite <- Ht. destruct Ps' as [_om Ps']. destruct Piom as [_s Piom].
-      apply protocol_generated with _om _s; try assumption. split; assumption.
-    }
-    assert (Hps : protocol_state_prop X s) by (exists oom; assumption).
-    destruct (decide (j = x)).
-    + subst x.
-      simpl in Ht.
-      destruct (vtransition (IM j) lx (s' j, iom)) as [si' om'] eqn:Hteq.
-      inversion Ht; subst. unfold composite_transition_item_projection_from_eq.
-      simpl.
-      rewrite state_update_eq in *.
-      simpl in Hv.
-      apply (finite_ptrace_extend Xj).
-      * apply IHHtr.
-        exists oom.
-        replace (@pair (@state message (@type message Xj)) (option message) si' oom)
-          with (vtransition (IM j) lx (s' j, iom)).
-        destruct Psj as [os'j Psj].
-        specialize (protocol_message_projection IM constraint j _ Piom); intros [sj HPjiom].
-        apply (protocol_generated Xj lx (s' j) os'j Psj sj iom HPjiom).
-        unfold valid; simpl.
-        exists s'.
-        split; try reflexivity.
-        split; try assumption.
-        split; try assumption.
-        destruct iom as [im|]
-        ; repeat split; assumption.
-      * assert
-          (Heqlx :
-            (@eq_rect_r index j (fun n : index => vlabel (IM n)) lx j (@eq_refl index j))
-            = lx
-          ) by reflexivity.
-        rewrite Heqlx.
-        specialize (protocol_message_projection IM constraint j _ Piom); intros HPjiom.
-        repeat split; try assumption.
-        exists s'.
-        repeat split; assumption.
-    + simpl in Ht. destruct (vtransition (IM x) lx (s' x, iom)) eqn:Hteq.
-      inversion Ht; subst.
-      rewrite state_update_neq in IHHtr; try assumption.
-      apply IHHtr.
-      assumption.
-Qed.
-
-Lemma protocol_state_projection
-  (s : state)
-  (Hps : protocol_state_prop X s)
-  : protocol_state_prop Xj (s j).
-Proof.
-  apply protocol_state_has_trace in Hps.
-  destruct Hps as [is [tr [[Htr His] Hs]]].
-  specialize (finite_trace_projection_last_state _ _ Htr) as Hlst.
-  apply _finite_ptrace_projection in Htr as Hptr.
-  - apply finite_ptrace_last_pstate in Hptr.
-    simpl in *.
-    rewrite Hlst in Hptr.
-    subst. assumption.
-  - apply initial_is_protocol. specialize (His j). assumption.
-Qed.
-
-(* The projection of a finite protocol trace remains a protocol trace *)
-
-Lemma finite_ptrace_projection
-  (s : vstate X)
-  (trx : list (vtransition_item X))
-  (Htr : finite_protocol_trace_from X s trx)
-   : finite_protocol_trace_from Xj (s j) (finite_trace_projection_list trx).
-Proof.
-  apply _finite_ptrace_projection; [|assumption].
-  apply protocol_state_projection.
-  apply finite_ptrace_first_pstate in Htr.
-  assumption.
-Qed.
-
-(* The projection of a preloaded finite protocol trace remains a preloaded protocol trace *)
-
-Lemma _preloaded_finite_ptrace_projection
-  (s : vstate X)
-  (Psj : protocol_state_prop (pre_loaded_with_all_messages_vlsm (IM j)) (s j))
-  (trx : list (vtransition_item X))
-  (Htr : finite_protocol_trace_from (pre_loaded_with_all_messages_vlsm X) s trx)
-   : finite_protocol_trace_from (pre_loaded_with_all_messages_vlsm (IM j)) (s j) (finite_trace_projection_list trx).
-Proof.
-  induction Htr.
-  - constructor. assumption.
-  - destruct l as [x lx]; simpl.
-    destruct H as [[Ps' [Piom [Hv Hc]]] Ht].
-    assert (Hpp : protocol_prop (pre_loaded_with_all_messages_vlsm X) (s, oom)).
-    { rewrite <- Ht. destruct Ps' as [_om Ps']. destruct Piom as [_s Piom].
-      apply protocol_generated with _om _s; try assumption. split; assumption.
-    }
-    assert (Hps : protocol_state_prop (pre_loaded_with_all_messages_vlsm X) s) by (exists oom; assumption).
-    destruct (decide (j = x)).
-    + subst x.
-      unfold vtransition in Ht. simpl in Ht.
-      unfold vtransition in Ht. simpl in Ht.
-      destruct (vtransition (IM j) lx (s' j, iom)) as [si' om'] eqn:Hteq.
-      inversion Ht; subst. 
-      unfold composite_transition_item_projection_from_eq. simpl.
-      rewrite state_update_eq in *.
-      simpl in Hv.
-      apply (finite_ptrace_extend (pre_loaded_with_all_messages_vlsm (IM j))).
-      * apply IHHtr.
-        exists oom.
-
-        replace
-          (@pair
-            (@state message
-              (@type message (@pre_loaded_with_all_messages_vlsm message (IM j))))
-            (option message)
-            si' oom)
-          with (vtransition (IM j) lx (s' j, iom)).
-        destruct Psj as [os'j Psj].
-        specialize (protocol_generated (pre_loaded_with_all_messages_vlsm (IM j)) lx (s' j) os'j Psj)
-          as Hgen.
-        specialize (Hgen (proj1_sig (vs0 (IM j))) iom).
-        spec Hgen; [apply (pre_loaded_with_all_messages_message_protocol_prop (IM j))|].
-        spec Hgen; [| apply Hgen].
-        assumption.
-      * assert
-          (Heqlx :
-            (@eq_rect_r index j (fun n : index => vlabel (IM n)) lx j (@eq_refl index j))
-            = lx
-          ) by reflexivity.
-        rewrite Heqlx.
-        split; [|assumption].
-        split; [assumption|].
-        split; [|assumption].
-        exists (proj1_sig (vs0 (IM j))).
-        apply (pre_loaded_with_all_messages_message_protocol_prop (IM j)).
-    + simpl in Ht. unfold vtransition in Ht.
-      simpl in Ht.
-      destruct (vtransition (IM x) lx (s' x, iom)) eqn:Hteq.
-      inversion Ht; subst.
-      rewrite state_update_neq in IHHtr by assumption.
-      apply IHHtr.
-      assumption.
-Qed.
-
-Lemma preloaded_protocol_state_projection
-  (s : state)
-  (Hps : protocol_state_prop (pre_loaded_with_all_messages_vlsm X) s)
-  : protocol_state_prop (pre_loaded_with_all_messages_vlsm (IM j)) (s j).
-Proof.
-  apply protocol_state_has_trace in Hps.
-  destruct Hps as [is [tr [[Htr His] Hs]]].
-  specialize (preloaded_finite_trace_projection_last_state _ _ Htr) as Hlst.
-  apply _preloaded_finite_ptrace_projection in Htr as Hptr.
-  - apply finite_ptrace_last_pstate in Hptr.
-    simpl in *.
-    rewrite Hlst in Hptr.
-    subst. assumption.
-  - apply initial_is_protocol. specialize (His j). assumption.
-Qed.
-
-Lemma preloaded_finite_ptrace_projection
-  (s : vstate X)
-  (trx : list (vtransition_item X))
-  (Htr : finite_protocol_trace_from (pre_loaded_with_all_messages_vlsm X) s trx)
-   : finite_protocol_trace_from (pre_loaded_with_all_messages_vlsm (IM j)) (s j) (finite_trace_projection_list trx).
-Proof.
-  apply _preloaded_finite_ptrace_projection; [|assumption].
-  apply preloaded_protocol_state_projection.
-  apply finite_ptrace_first_pstate in Htr.
-  assumption.
-Qed.  
-
-Lemma in_futures_projection
-  (s1 s2 : state)
-  (Hfutures : in_futures X s1 s2)
-  : in_futures Xj (s1 j) (s2 j).
-Proof.
-  destruct Hfutures as [tr [Htr Hs2]].
-  specialize (finite_ptrace_projection s1 tr Htr); intros Htrj.
-  exists (finite_trace_projection_list tr).
-  split; [assumption|].
-  subst s2.
-  apply finite_trace_projection_last_state.
-  assumption.
-Qed.
-
-Definition in_projection
-   (tr : Stream (composite_transition_item IM))
-   (n : nat)
-   := from_projection (Str_nth n tr).
-
-Definition in_projection_dec
-  := forall (tr : Stream (composite_transition_item IM)),
-       bounding (in_projection tr)
-       + { ss : monotone_nat_stream
-         | filtering_subsequence from_projection tr ss
-         }.
-
-Definition infinite_trace_projection_stream
-  (ss: Stream (composite_transition_item IM))
-  (ks: monotone_nat_stream)
-  (Hfilter: filtering_subsequence from_projection ss ks)
-  : Stream (vtransition_item (IM j))
-  :=
-  let subs := stream_subsequence ss ks in
-  let HForAll := stream_filter_Forall from_projection ss ks Hfilter in
-  let subsP := stream_annotate from_projection subs HForAll in
-  Streams.map
-    (fun item : {a : vtransition_item X | from_projection a} =>
-      let (item, e) := item in
-      let lj := eq_rect_r _ (projT2 (l item)) e in
-      @Build_transition_item _ (type Xj) lj (input item) (destination item j) (output item)
+Lemma transition_sub_projection
+  l s om s' om'
+  (Ht : composite_transition IM l  (s, om) = (s', om'))
+  (Hsub : sub_index_prop (projT1 l))
+  : composite_transition sub_IM
+    (existT (fun n : sub_index => vlabel (sub_IM n))
+      (dec_exist _ (projT1 l) Hsub)
+      (projT2 l)
     )
-    subsP.
-
-Lemma finite_trace_projection_stream
-  (ss: Stream (composite_transition_item IM))
-  (ks: monotone_nat_stream)
-  (Hfilter: filtering_subsequence from_projection ss ks)
-  (n : nat)
-  (kn := Str_nth n (proj1_sig ks))
-  (ss_to_kn := stream_prefix ss (succ kn))
-  (sproj := infinite_trace_projection_stream ss ks Hfilter)
-  : stream_prefix sproj (succ n) = finite_trace_projection_list ss_to_kn.
+    (composite_state_sub_projection s, om)
+    = (composite_state_sub_projection s', om').
 Proof.
-  unfold sproj. unfold infinite_trace_projection_stream.
-  rewrite <- stream_prefix_map.
-  specialize
-    (stream_prefix_annotate
-      from_projection
-      (stream_subsequence ss ks)
-      (stream_filter_Forall from_projection ss ks Hfilter)
-      (succ n)
-    ); intros [Hall Heq].
-  clear -Heq.
+  simpl. simpl in Ht.
+  destruct l as (i, li).
+  unfold vtransition. simpl.
+  unfold composite_state_sub_projection at 1. simpl.
+  destruct (vtransition (IM i) li (s i, om)) as (si', omi') eqn:Hti.
+  inversion Ht. subst omi' s'. clear Ht.
   match goal with
-  |- List.map _ ?s = _ => replace s with
-      (list_annotate from_projection (stream_prefix (stream_subsequence ss ks) (succ n)) Hall)
+  |- (let (_, _) := ?t in _) = _ =>
+    replace t with (si', om')
   end.
-  specialize
-    (stream_filter_prefix
-       ss
-       ks
-       Hfilter
-       n
-    ); intros Hsfilter.
-  remember stream_prefix as sp.
-  simpl in Hsfilter. subst.
-  unfold succ in *.
-  generalize dependent Hall.
-  rewrite Hsfilter.
-  intros.
-  unfold ss_to_kn. unfold kn.
-  apply finite_trace_projection_list_alt_iff.
+  f_equal.
+  apply functional_extensionality_dep.
+  intro sub_j. unfold sub_index in sub_j.
+  destruct_dec_sig sub_j j Hj Heqj.
+  subst sub_j. unfold composite_state_sub_projection at 2.
+  destruct (decide (j = i)).
+  - subst.
+    simpl. rewrite state_update_eq.
+    apply sub_IM_state_update_eq.
+  - rewrite! state_update_neq; [reflexivity|assumption|].
+    intro contra. apply dec_sig_eq_iff in contra. contradiction.
 Qed.
 
-Definition trace_projection
-  (Hproj_dec : in_projection_dec)
-  (tr : vTrace X)
-  : vTrace (IM j).
+Lemma valid_sub_projection
+  l s om
+  (Hv : composite_valid IM l  (s, om))
+  (Hsub : sub_index_prop (projT1 l))
+  : composite_valid sub_IM
+    (existT (fun n : sub_index => vlabel (sub_IM n))
+      (dec_exist _ (projT1 l) Hsub)
+      (projT2 l)
+    )
+    (composite_state_sub_projection s, om).
 Proof.
-  destruct tr as [s ls | s ss].
-  - exact (Finite (s j) (finite_trace_projection_list ls)).
-  - specialize (Hproj_dec ss).
-    destruct Hproj_dec as [[n1 _] | [ks Hfilter]].
-    + exact (Finite (s j) (finite_trace_projection_list (stream_prefix ss n1))).
-    + exact (Infinite (s j) (infinite_trace_projection_stream ss ks Hfilter)).
-Defined.
-
-Lemma trace_projection_initial_state
-  (Hproj_dec : in_projection_dec)
-  (tr : vTrace X)
-  : trace_first (trace_projection Hproj_dec tr)
-  = trace_first tr j.
-Proof.
-  destruct tr; try reflexivity.
-  simpl.
-  destruct (Hproj_dec s0).
-  - destruct b; reflexivity.
-  - destruct s1; reflexivity.
+  simpl. simpl in Hv.
+  destruct l as (i, li).
+  assumption.
 Qed.
 
-Lemma infinite_ptrace_projection
-  (s: vstate X)
-  (ss: Stream transition_item)
-  (Psj: protocol_state_prop Xj (s j))
-  (Htr: infinite_protocol_trace_from X s ss)
-  (fs : monotone_nat_stream)
-  (Hfs: filtering_subsequence from_projection ss fs)
-  : infinite_protocol_trace_from Xj (s j) (infinite_trace_projection_stream ss fs Hfs).
-Proof.
-  apply infinite_protocol_trace_from_prefix_rev.
-  specialize (infinite_protocol_trace_from_prefix X s ss Htr); intro Hftr.
-  intros [| n].
-  - constructor. assumption.
-  - rewrite finite_trace_projection_stream.
-    apply finite_ptrace_projection; try assumption.
-    apply Hftr.
-Qed.
+Definition composite_state_sub_projection_lift
+  (ss : composite_state sub_IM)
+  (i : index)
+  :=
+  match (decide (sub_index_prop i)) with
+  | left e => ss (dec_exist _ i e)
+  | _ => proj1_sig (composite_s0 IM) i
+  end. 
 
-(* The projection of an protocol trace remains a protocol trace *)
+Definition sub_constraint
+  (l : composite_label sub_IM)
+  (som : composite_state sub_IM * option message)
+  : Prop
+  :=
+  let i := proj1_sig (projT1 l) in
+  let li := projT2 l in
+  let lx : composite_label IM := (existT (fun i : index => vlabel (IM i)) i li) in
+  let (ss, om) := som in
+  let s := composite_state_sub_projection_lift ss in
+  constraint lx (s, om).
 
-Lemma ptrace_from_projection
-  (Hproj_dec : in_projection_dec)
-  (tr : vTrace X)
-  (Psj : protocol_state_prop Xj (trace_first tr j))
-  (Htr : ptrace_from_prop X tr)
-   : ptrace_from_prop Xj (trace_projection Hproj_dec tr).
-Proof.
-  destruct tr as [s ls | s ss].
-  - apply finite_ptrace_projection; assumption.
-  - simpl. destruct (Hproj_dec ss) as [[n _]|Hinf].
-    + apply finite_ptrace_projection; try assumption.
-      apply infinite_protocol_trace_from_prefix. assumption.
-    + destruct Hinf as [ks HFilter].
-      apply infinite_ptrace_projection; assumption.
-Qed.
-
-Lemma protocol_trace_projection
-  (Hproj_dec : in_projection_dec)
-  (tr : vTrace X)
-  (Htr : protocol_trace_prop X tr)
-  : protocol_trace_prop Xj (trace_projection Hproj_dec tr).
-Proof.
-  assert (Hfrom := protocol_trace_from X tr Htr).
-  assert (Hinit := protocol_trace_initial X tr Htr).
-  apply protocol_trace_from_iff.
-  split.
-  - apply ptrace_from_projection; try assumption.
-    apply protocol_state_prop_iff.
-    left.
-    apply (initial_state_projection IM constraint j) in Hinit.
-    exists (exist _ _ Hinit).
-    reflexivity.
-  - rewrite trace_projection_initial_state.
-    apply initial_state_projection.
-    assumption.
-Qed.
-
-(* We axiomatize projection friendliness as the converse of protocol_trace_projection *)
-Definition finite_projection_friendly
-  := forall
-    (sj : vstate (IM j))
-    (trj : list (vtransition_item (IM j)))
-    (Htrj : finite_protocol_trace Xj sj trj),
-    exists (sx : vstate X) (trx : list (vtransition_item X)),
-      finite_protocol_trace X sx trx
-      /\ sx j = sj
-      /\ finite_trace_projection_list trx = trj.
-
-Definition projection_friendly
-  (Hproj_dec : in_projection_dec)
-  := forall
-  (trj : vTrace (IM j))
-  (Htrj : protocol_trace_prop Xj trj),
-  exists (tr : vTrace X),
-    protocol_trace_prop X tr
-    /\ trace_projection Hproj_dec tr = trj.
-
-Lemma projection_friendly_finite
-  (Hproj_dec : in_projection_dec)
-  (Hfr : projection_friendly Hproj_dec)
-  : finite_projection_friendly.
-Proof.
-  unfold finite_projection_friendly;  intros.
-  specialize (Hfr (Finite sj trj) Htrj).
-  destruct Hfr as [[s tr| s tr] [Htr Heq]].
-  + exists s. exists tr.
-    split; try assumption.
-    unfold trace_projection in Heq.
-    inversion Heq.
-    split; reflexivity.
-  + unfold trace_projection in Heq.
-    destruct (Hproj_dec tr) as [[n1 _] | (ks, Hfilter)]; inversion Heq.
-    subst; clear Heq.
-    exists s. exists (stream_prefix tr n1).
-    destruct Htr as [Htr Hinit].
-    repeat split; try reflexivity; try assumption.
-    apply infinite_protocol_trace_from_prefix.
-    assumption.
-Qed.
-
-Lemma projection_friendly_in_futures'
-  (sx: state)
-  (trx: list transition_item)
-  (Htrx: finite_protocol_trace X sx trx)
-  (sj: state)
-  (Hsx: sx j = sj)
-  (Hall: Forall from_projection
-         (filter (fun a => bool_decide (from_projection a)) trx))
-  (s1 s2: state)
-  (n1 n2: nat)
-  (Hle: n1 <= n2)
-  (Hs1: nth_error
-        (sj
-         :: List.map destination (finite_trace_projection_list_alt trx Hall))
-        n1 = Some s1)
-  (Hs2: nth_error
-        (sj
-         :: List.map destination (finite_trace_projection_list_alt trx Hall))
-        n2 = Some s2)
-  : exists sX1 sX2 : vstate X, sX1 j = s1 /\ sX2 j = s2 /\ in_futures X sX1 sX2.
-Proof.
-    assert
-      (HsX1 :
-        exists (nX1 nX2 : nat) (sX1 sX2 : vstate X),
-          nX1 <= nX2 /\ sX1 j = s1 /\ sX2 j = s2
-          /\ nth_error (sx :: List.map destination trx) nX1 = Some sX1
-          /\ nth_error (sx :: List.map destination trx) nX2 = Some sX2
-      ).
-    {
-      destruct n1; destruct n2.
-      - exists 0; exists 0; exists sx; exists sx
-        ; inversion Hs1; inversion Hs2; subst; repeat split; assumption.
-      - exists 0; inversion Hs1; clear Hs1; subst.
-        simpl in Hs2.
-        rewrite nth_error_map in Hs2.
-        unfold finite_trace_projection_list_alt in Hs2.
-        rewrite nth_error_map in Hs2.
-        specialize
-          (nth_error_list_annotate
-            from_projection
-            (filter (fun a => bool_decide (from_projection a)) trx)
-            Hall
-            n2
-          ); intros [oitem [Hoa Hnth]].
-        match type of Hs2 with
-        | option_map _ (option_map _ ?n) = _ => replace n with oitem in Hs2
-        end.
-        clear Hoa.
-        destruct oitem as [[item Hitem]|]; try inversion Hs2; subst; clear Hs2.
-        simpl in Hnth.
-        symmetry in Hnth.
-        apply nth_error_filter in Hnth.
-        destruct Hnth as [nX2 [Hindex Hnth]].
-        exists (S nX2).
-        exists sx.
-        exists (destination item).
-        repeat split.
-        + lia.
-        + simpl. rewrite nth_error_map.
-          replace
-            (@nth_error (@transition_item message (@composite_type message index IM)) trx nX2)
-            with (Some item).
-          reflexivity.
-      - inversion Hle.
-      - simpl in Hs1. simpl in Hs2.
-        rewrite nth_error_map in Hs1.
-        rewrite nth_error_map in Hs2.
-        unfold finite_trace_projection_list_alt in Hs1.
-        unfold finite_trace_projection_list_alt in Hs2.
-        rewrite nth_error_map in Hs1.
-        rewrite nth_error_map in Hs2.
-        specialize
-          (nth_error_list_annotate
-            from_projection
-            (filter (fun a => bool_decide (from_projection a)) trx)
-            Hall
-            n2
-          ); intros [oitem2 [Hoa2 Hn2th]].
-        specialize
-          (nth_error_list_annotate
-            from_projection
-            (filter (fun a => bool_decide (from_projection a)) trx)
-            Hall
-            n1
-          ); intros [oitem1 [Hoa1 Hn1th]].
-        match type of Hs2 with
-        | option_map _ (option_map _ ?n) = _ => replace n with oitem2 in Hs2
-        end.
-        match type of Hs1 with
-        | option_map _ (option_map _ ?n) = _ => replace n with oitem1 in Hs1
-        end.
-        clear Hoa1.
-        destruct oitem2 as [[item2 Hitem2]|]; try inversion Hs2; subst; clear Hs2.
-        destruct oitem1 as [[item1 Hitem1]|]; try inversion Hs1; subst; clear Hs1.
-        simpl in Hn1th.
-        simpl in Hn2th.
-        symmetry in Hn1th.
-        symmetry in Hn2th.
-        apply nth_error_filter in Hn1th.
-        apply nth_error_filter in Hn2th.
-        destruct Hn2th as [nX2 [Hindex2 Hn2th]].
-        destruct Hn1th as [nX1 [Hindex1 Hn1th]].
-        exists (S nX1).
-        exists (S nX2).
-        exists (destination item1).
-        exists (destination item2).
-        repeat split; try assumption.
-        + assert (Hle' : n1 <= n2) by lia.
-          specialize (nth_error_filter_index_le _ _ _ _ Hle' _ _ Hindex1 Hindex2).
-          intro; lia.
-        + simpl. rewrite nth_error_map.
-          replace (@nth_error (@transition_item message (@composite_type message index IM)) trx nX1)
-            with (Some item1).
-          reflexivity.
-        + simpl. rewrite nth_error_map.
-          replace (@nth_error (@transition_item message (@composite_type message index IM)) trx nX2)
-            with (Some item2).
-          reflexivity.
-    }
-    destruct HsX1 as [nX1 [nX2 [sX1 [sX2 [HleX [Hps1 [Hps2 [HsX1 HsX2]]]]]]]].
-    exists sX1. exists sX2. repeat split; try assumption.
-    specialize (in_futures_witness_reverse X sX1 sX2 (exist (protocol_trace_prop X) (Finite sx trx) Htrx) nX1 nX2 HleX HsX1 HsX2).
-    intros; assumption.
-Qed.
-
-Lemma projection_friendly_in_futures
-  (Hfr : finite_projection_friendly)
-  (s1 s2 : vstate (IM j))
-  (Hfuture : in_futures Xj s1 s2)
-  : exists (sX1 sX2 : vstate X),
-    sX1 j = s1 /\ sX2 j = s2 /\ in_futures X sX1 sX2.
-Proof.
-  specialize (in_futures_witness Xj s1 s2 Hfuture)
-  ; intros [trj [n1 [n2 [Hle [Hs1 Hs2]]]]].
-  clear Hfuture.
-  destruct trj as [trj Htrj].
-  specialize (trace_prefix_fn_protocol Xj trj Htrj n2); intros Hpref.
-  remember (trace_prefix_fn Xj trj n2) as trj2.
-  destruct trj2 as [sj' lj' | sj' lj']; destruct trj as [sj lj | sj lj]
-  ; inversion Heqtrj2
-  ; subst sj' lj'.
-  - specialize (Hfr sj (list_prefix lj n2) Hpref).
-    destruct Hfr as [sx [trx [Htrx [Hsx Hproj]]]].
-    assert (Hall : Forall from_projection
-              (filter (fun a => bool_decide (from_projection a)) trx))
-      by apply filter_Forall.
-    specialize (finite_trace_projection_list_alt_iff trx Hall); intro Heq.
-    rewrite <- Heq in Hproj.
-    simpl in Hs1.
-    simpl in Hs2.
-    assert
-      (Hs1' :
-        nth_error (sj :: List.map destination lj) n1 =
-        nth_error (sj :: List.map destination (list_prefix lj n2)) n1
-      ).
-    { destruct n1; try reflexivity. simpl.
-      rewrite list_prefix_map.
-      symmetry. apply list_prefix_nth. assumption.
-    }
-    assert
-      (Hs2' :
-        nth_error (sj :: List.map destination lj) n2 =
-        nth_error (sj :: List.map destination (list_prefix lj n2)) n2
-      ).
-    { destruct n2; try reflexivity. simpl.
-      rewrite list_prefix_map.
-      symmetry. apply list_prefix_nth. constructor.
-    }
-    apply projection_friendly_in_futures' with sx trx sj Hall n1 n2; try assumption
-    ; rewrite Hproj.
-    + rewrite <- Hs1. symmetry. assumption.
-    + rewrite <- Hs2. symmetry. assumption.
-  - specialize (Hfr sj (stream_prefix lj n2) Hpref).
-    destruct Hfr as [sx [trx [Htrx [Hsx Hproj]]]].
-    assert (Hall : Forall from_projection
-              (filter (fun a => bool_decide (from_projection a)) trx))
-      by apply filter_Forall.
-    specialize (finite_trace_projection_list_alt_iff trx Hall); intro Heq.
-    rewrite <- Heq in Hproj.
-    simpl in Hs1.
-    simpl in Hs2.
-    assert
-      (Hs1' :
-        Some (Str_nth n1 (Cons sj (map destination lj))) =
-        nth_error (sj :: List.map destination (stream_prefix lj n2)) n1
-      ).
-    { destruct n1; try reflexivity. simpl.
-      rewrite stream_prefix_map.
-      rewrite stream_prefix_nth; try assumption.
-      reflexivity.
-    }
-    assert
-      (Hs2' :
-      Some (Str_nth n2 (Cons sj (map destination lj))) =
-        nth_error (sj :: List.map destination (stream_prefix lj n2)) n2
-      ).
-    { destruct n2; try reflexivity.
-      rewrite stream_prefix_map.
-      remember (S n2) as sn2. rewrite Heqsn2 at 3.
-      simpl.
-      rewrite stream_prefix_nth; subst; constructor.
-    }
-    apply projection_friendly_in_futures' with sx trx sj Hall n1 n2; try assumption
-    ; rewrite Hproj; rewrite <- Hs1 || rewrite <- Hs2; symmetry; assumption.
-Qed.
-
-End ProjectionTraces.
-
-Section ProjectionTraces_membership.
+Existing Instance X_has_been_sent_capability.
 
 Context
-  {message : Type}
-  {index : Type}
-  {IndEqDec : EqDecision index}
-  (IM : index -> VLSM message)
-  {i0 : Inhabited index}
-  (constraint : composite_label IM -> composite_state IM * option message -> Prop)
-  (X := composite_vlsm IM constraint)
+  (seed : message -> Prop)
+  (Hno_equiv : constraint_subsumption IM constraint (no_equivocations Free))
+  (seeded_constraint : composite_label sub_IM -> composite_state sub_IM * option message -> Prop)
+  (Xj := composite_no_equivocation_vlsm_with_pre_loaded sub_IM (free_constraint sub_IM) sub_has_been_sent_capabilities finite_sub_index seed)
   .
 
-Lemma finite_trace_projection_list_in
-  (tr : list (vtransition_item X))
-  (itemX : vtransition_item X)
-  (HitemX : In itemX tr)
-  (j := projT1 (l itemX))
-  : In (@Build_transition_item _ (type (IM j)) (projT2 (l itemX)) (input itemX) (destination itemX j) (output itemX)) (finite_trace_projection_list IM j tr).
-Proof.
-  induction tr; [inversion HitemX|].
-  destruct HitemX as [HitemX | HitemX].
-  - simpl. subst a. unfold j in *. clear j.
-    match goal with
-    |- context [decide ?eq] => destruct (decide eq)
-    end
-    ; [| elim n; reflexivity].
-    left.
-    f_equal.
-    replace e with (@eq_refl index (projT1 (l itemX))) by apply UIP.
-    reflexivity.
-  - spec IHtr HitemX.
-    simpl.
-    match goal with
-    |- context [decide ?eq] => destruct (decide eq)
-    end
-    ;[|assumption].
-    right. assumption.
-Qed.
 
-Lemma finite_trace_projection_list_in_rev
-  (tr : list (composite_transition_item IM))
-  (j : index)
-  (itemj : vtransition_item (IM j))
-  (Hitemj : In itemj  (finite_trace_projection_list IM j tr))
-  : exists
-    (itemX : composite_transition_item IM)
-    (Houtput : output itemX = output itemj)
-    (Hinput : input itemX = input itemj)
-    (Hl1 : j = projT1 (l itemX))
-    (Hl2 : eq_rect_r _ (projT2 (l itemX)) Hl1 = l itemj)
-    (Hdestination : destination itemX j = destination itemj),
-    In itemX tr.
+Lemma Xj_incl_Pre_Sub_Free
+  : VLSM_incl Xj (pre_loaded_with_all_messages_vlsm Sub_Free).
 Proof.
-  induction tr; [contradict Hitemj|].
-  simpl in Hitemj.
-  match type of Hitemj with
-  | context [decide ?eq] => destruct (decide eq)
+  subst Xj.
+  unfold composite_no_equivocation_vlsm_with_pre_loaded.
+  specialize
+    (preloaded_constraint_subsumption_pre_loaded_with_all_messages_incl sub_IM
+      (no_equivocations_additional_constraint_with_pre_loaded sub_IM
+        (free_constraint sub_IM) sub_has_been_sent_capabilities
+        finite_sub_index seed)
+      (free_constraint sub_IM)
+    ) as Hincl.
+  spec Hincl; [intros s Hs l om H; exact I|].
+  match goal with
+  |- context [pre_loaded_with_vlsm ?v _] =>
+    apply VLSM_incl_trans with (machine (pre_loaded_with_all_messages_vlsm v))
+  end
+  ; [| apply Hincl].
+  clear Hincl.
+  match goal with
+  |- context [pre_loaded_with_all_messages_vlsm ?v] =>
+    apply VLSM_incl_trans with (machine (pre_loaded_with_vlsm v (fun m => True)))
   end.
-  - destruct Hitemj as [Hitemj | Hitemj].
-    + subst itemj. simpl. exists a. exists eq_refl. exists eq_refl. exists e.
-      exists eq_refl. exists eq_refl. left. reflexivity.
-    + spec IHtr Hitemj.
-      destruct IHtr as [itemX [Houtput [Hinput [Hl1 [Hl2 [Hdestination HitemX]]]]]].
-      exists itemX. repeat split; [assumption| assumption |].
-      exists Hl1. exists Hl2. exists Hdestination. right. assumption.
-  - spec IHtr Hitemj.
-    destruct IHtr as [itemX [Houtput [Hinput [Hl1 [Hl2 [Hdestination HitemX]]]]]].
-    exists itemX. repeat split; [assumption| assumption |].
-    exists Hl1. exists Hl2. exists Hdestination. right. assumption.
+  - match goal with
+    |- context [pre_loaded_with_vlsm ?v _] => 
+      apply (pre_loaded_with_vlsm_incl v seed (fun m => True))
+    end.
+    intuition.
+  - match goal with
+    |- context [pre_loaded_with_all_messages_vlsm ?v] => 
+      specialize (pre_loaded_with_all_messages_vlsm_is_pre_loaded_with_True v) as Hincl
+    end.
+    apply VLSM_eq_incl_iff in Hincl.
+    apply proj2 in Hincl.
+    assumption.
 Qed.
 
-End ProjectionTraces_membership.
+Definition trace_sub_item_input_is_seeded_or_sub_previously_sent
+  (tr : list (composite_transition_item IM))
+  : Prop
+  :=
+  forall pre item suf m,
+    tr = pre ++ [item] ++ suf ->
+    input item = Some m ->
+    from_sub_projection item ->
+    seed m \/ exists pre_item, In pre_item pre /\ output pre_item = Some m /\ from_sub_projection pre_item.
+
+Definition state_sub_item_input_is_seeded_or_sub_previously_sent
+  (s : composite_state IM)
+  : Prop
+  := forall is tr,
+    finite_protocol_trace Pre is tr ->
+    last (map destination tr) is = s ->
+    trace_sub_item_input_is_seeded_or_sub_previously_sent tr.
+
+Lemma finite_protocol_trace_sub_projection
+  (s : composite_state IM)
+  (tr : list (composite_transition_item IM))
+  (Hmsg :  trace_sub_item_input_is_seeded_or_sub_previously_sent tr)
+  (Htr : finite_protocol_trace X s tr)
+  : finite_protocol_trace Xj (composite_state_sub_projection s) (finite_trace_sub_projection tr).
+Proof.
+  destruct Htr as [Htr His].
+  apply (composite_initial_state_sub_projection s) in His.
+  split; [|assumption].
+  apply (initial_is_protocol Xj) in His as Hisp.
+  induction tr using rev_ind; simpl
+  ; [constructor; assumption|].
+  apply finite_protocol_trace_from_app_iff in Htr.
+  destruct Htr as [Htr Hx].
+  spec IHtr.
+  { intros pre item suf m Heq Hin_m Hitem.
+    subst tr.
+    specialize (Hmsg pre item (suf ++ [x]) m).
+    rewrite! app_assoc in Hmsg.
+    specialize (Hmsg eq_refl Hin_m Hitem).
+    destruct Hmsg as [Hseed | Hmsg]
+    ; [left | right] ; assumption.
+  }
+  spec IHtr Htr.
+  rewrite finite_trace_sub_projection_app.
+  apply finite_protocol_trace_from_app_iff.
+  split; [assumption|].
+  specialize (Hmsg tr x []).
+  match goal with 
+  |- finite_protocol_trace_from _ ?l _ => remember l as lst
+  end.
+  assert (Hlst : protocol_state_prop Xj lst).
+  { apply finite_ptrace_last_pstate in IHtr. subst. assumption. }
+  simpl.
+  destruct (decide (from_sub_projection x))
+  ;[|constructor; assumption].
+  apply (finite_ptrace_singleton Xj).
+  inversion Hx. subst x tl. simpl in *.
+  destruct H3 as [Hv Ht].
+  specialize (transition_sub_projection _ _ _ _ _ Ht f)
+    as Htj.
+  destruct Hv as [_ [_ [Hv Hc]]].
+  specialize (valid_sub_projection _ _ _ Hv f)
+    as Hvj.
+  rewrite <- H1 in Htj, Hvj.
+  assert (Hlst' : composite_state_sub_projection s' = lst).
+  { subst lst s'. symmetry.
+    apply finite_trace_sub_projection_last_state. assumption.
+  }
+  rewrite Hlst' in Htj, Hvj.
+  repeat split; [assumption | | assumption | | assumption].
+  - destruct iom as [m|]; [|apply (option_protocol_message_None Xj)].
+    apply (option_protocol_message_Some Xj).
+    specialize (Hmsg m eq_refl eq_refl f).
+    destruct Hmsg as [Hseed | [item [Hitem [Hout Hsub_item]]]]
+    ; [apply (initial_message_is_protocol Xj); right; assumption|].
+    specialize (finite_trace_sub_projection_list_in tr item Hitem Hsub_item)
+      as Hin_sub.
+    apply (protocol_trace_output_is_protocol Xj _ _ IHtr).
+    apply Exists_exists. eexists _. split; [apply Hin_sub|].
+    assumption.
+  - apply Hno_equiv in Hc.
+    destruct iom as [m|]; [|exact I].
+    simpl in *.
+    specialize (Hmsg m eq_refl eq_refl f).
+    destruct Hmsg as [Hseed | [item [Hitem [Hout Hsub_item]]]]
+    ; [right; right; assumption|].
+    left.
+    specialize (proper_sent Sub_Free lst) as Hproper.
+    assert (Hlstp : protocol_state_prop (pre_loaded_with_all_messages_vlsm Sub_Free) lst).
+    { apply VLSM_incl_protocol_state with (MX := machine Xj); [|assumption].
+      apply Xj_incl_Pre_Sub_Free.
+    }
+    spec Hproper Hlstp.
+    apply Hproper.
+    apply has_been_sent_consistency; [apply Sub_Free_has_been_sent_capability| assumption| ].
+    exists (composite_state_sub_projection s), (finite_trace_sub_projection tr).
+    split.
+    { apply (VLSM_incl_finite_protocol_trace _ _ Xj_incl_Pre_Sub_Free).
+      split; assumption.
+    }
+    symmetry in Heqlst.
+    exists Heqlst.
+    apply Exists_exists. exists (composite_transition_item_sub_projection item Hsub_item).
+    split; [|assumption].
+    apply finite_trace_sub_projection_list_in. assumption.
+Qed.
+
+Lemma protocol_state_sub_projection
+  (s : state)
+  (Hs : state_sub_item_input_is_seeded_or_sub_previously_sent s)
+  (Hps : protocol_state_prop X s)
+  : protocol_state_prop Xj (composite_state_sub_projection s).
+Proof.
+  apply protocol_state_has_trace in Hps.
+  destruct Hps as [is [tr [Htr Hlst]]].
+  specialize (finite_trace_sub_projection_last_state _ _ (proj1 Htr)) as Hlst'.
+  apply finite_protocol_trace_sub_projection in Htr as Hptr.
+  - destruct Hptr as [Hptr _]. apply finite_ptrace_last_pstate in Hptr.
+    simpl in *.
+    rewrite Hlst' in Hptr.
+    subst. assumption.
+  - unfold state_sub_item_input_is_seeded_or_sub_previously_sent in Hs.
+    apply Hs with is; [|assumption].
+    apply VLSM_incl_finite_protocol_trace; [|assumption].
+    apply X_incl_Pre.
+Qed.
+
+Lemma finite_protocol_trace_from_sub_projection
+  (s : composite_state IM)
+  (tr : list (composite_transition_item IM))
+  (lst := last (map destination tr) s)
+  (Hmsg : state_sub_item_input_is_seeded_or_sub_previously_sent lst)
+  (Htr : finite_protocol_trace_from X s tr)
+  : finite_protocol_trace_from Xj (composite_state_sub_projection s) (finite_trace_sub_projection tr).
+Proof.
+  apply finite_protocol_trace_from_complete_left in Htr.
+  destruct Htr as [is [pre [Htr Hs]]].
+  assert (Hpre := proj1 Htr).
+  apply finite_protocol_trace_from_app_iff in Hpre.
+  destruct Hpre as [Hpre _].
+  specialize (finite_trace_sub_projection_last_state _ _ Hpre) as Hpre_lst.
+  apply finite_protocol_trace_sub_projection in Htr.
+  - destruct Htr as [Htr His].
+    rewrite finite_trace_sub_projection_app in Htr.
+    apply finite_protocol_trace_from_app_iff in Htr.
+    destruct Htr as [_ Htr].
+    subst s. simpl in *.
+    rewrite Hpre_lst in Htr. assumption.
+  - specialize (Hmsg is (pre ++ tr)).
+    apply Hmsg.
+    + apply VLSM_incl_finite_protocol_trace; [|assumption].
+      apply X_incl_Pre.
+    + rewrite map_app, last_app. subst lst s. reflexivity.
+Qed.
+
+Lemma in_futures_sub_projection
+  (s1 s2 : state)
+  (Hs2 : state_sub_item_input_is_seeded_or_sub_previously_sent s2)
+  (Hfutures : in_futures X s1 s2)
+  : in_futures Xj (composite_state_sub_projection s1) (composite_state_sub_projection s2).
+Proof.
+  destruct Hfutures as [tr [Htr Heq_s2]]. subst s2.
+  specialize (finite_protocol_trace_from_sub_projection s1 tr Hs2 Htr); intros Htrj.
+  exists (finite_trace_sub_projection tr).
+  split; [assumption|].
+  apply finite_trace_sub_projection_last_state.
+  assumption.
+Qed.
+
+End sub_projection_with_no_equivocation_constraints.
+End sub_composition.
